Add Client.Encrypt
Add new files:
 - SDK/Client.dfy
 - SDK/MessageBody.dfy

Include previously written files
 - HKDF/CryptoMac.dfy
 - HKDF/HKDF.dfy
 - HKDF/HKDFSpec.dfy
 - Util/Arrays.dfy

Move extern files into extern/dotnet folder:
 - Arrays-extern.cs
 - HKDF-extern.cs

Modify Main.dfy to test the new Client.Encrypt.

Rename array_of_seq to SeqToArray in StandardLibrary.

Make StringWriter.data non-ghost. This is a temporary solution, as a step toward making StringWriter store the characters written at run time.

Update test files with the new location of extern C# code. This includes two new macros in lit.site.cfg.

Strengthen postcondition of CMM.GetEncryptionMaterials to say something about the validity of the signing key.
Add postcondition to EncryptionMaterials to say that given signing key has been placed in field.

Uint.dfy:
Add constant UINT32_LIMIT.
Add methods to convert between uint64 and seq<byte>.

src/SDK/Materials.dfy
@@ -40,8 +40,9 @@ module Materials {
     predicate Valid()
       reads this
     {
-      (|encryptedDataKeys| > 0 ==> plaintextDataKey.Some?) &&
-      (plaintextDataKey.None? || ValidPlaintextDataKey(plaintextDataKey.get))
+      && (|encryptedDataKeys| != 0 ==> plaintextDataKey.Some?)
+      && (plaintextDataKey.None? || ValidPlaintextDataKey(plaintextDataKey.get))
+      && (forall i :: 0 <= i < |encryptedDataKeys| ==> encryptedDataKeys[i].Valid())
     }
 
     predicate ValidPlaintextDataKey(pdk: seq<uint8>)
@@ -56,12 +57,14 @@ module Materials {
                 plaintextDataKey: Option<seq<uint8>>,
                 signingKey: Option<seq<uint8>>)
       requires |encryptedDataKeys| > 0 ==> plaintextDataKey.Some?
+      requires forall i :: 0 <= i < |encryptedDataKeys| ==> encryptedDataKeys[i].Valid()
       requires plaintextDataKey.None? || |plaintextDataKey.get| == algorithmSuiteID.KeyLength()
       ensures Valid()
       ensures this.algorithmSuiteID == algorithmSuiteID
       ensures this.encryptedDataKeys == encryptedDataKeys
       ensures this.encryptionContext == encryptionContext
       ensures this.plaintextDataKey == plaintextDataKey
+      ensures this.signingKey == signingKey
     {
       this.algorithmSuiteID := algorithmSuiteID;
       this.encryptedDataKeys := encryptedDataKeys;
@@ -82,7 +85,7 @@ module Materials {
     }
 
     method AppendEncryptedDataKey(edk: EncryptedDataKey)
-      requires Valid()
+      requires Valid() && edk.Valid()
       requires plaintextDataKey.Some?
       modifies `encryptedDataKeys
       ensures Valid()
