src/SDK/Client.dfy
@@ -1,0 +1,123 @@
+include "../StandardLibrary/StandardLibrary.dfy"
+include "../StandardLibrary/UInt.dfy"
+include "Materials.dfy"
+include "CMM/Defs.dfy"
+include "MessageHeader.dfy"
+include "MessageBody.dfy"
+include "Serialize.dfy"
+include "../Crypto/Random.dfy"
+include "../Util/Streams.dfy"
+include "../Crypto/Digests.dfy"
+include "../Crypto/HKDF/HKDF.dfy"
+include "../Crypto/AESEncryption.dfy"
+include "../Crypto/Signature.dfy"
+
+module ESDKClient {
+  import opened StandardLibrary
+  import opened UInt = StandardLibrary.UInt
+  import Materials
+  import AlgorithmSuite
+  import CMMDefs
+  import Msg = MessageHeader
+  import MessageBody
+  import Serialize
+  import Random
+  import Digests
+  import Streams
+  import HKDF
+  import AESEncryption
+  import Signature
+
+  /*
+   * Encrypt a plaintext and serialize it into a message.
+   * Following https://github.com/awslabs/aws-encryption-sdk-specification/blob/master/client-apis/encrypt.md, 2019-09-24.
+   */
+  method Encrypt(plaintext: seq<uint8>, cmm: CMMDefs.CMM, encryptionContext: Materials.EncryptionContext) returns (res: Result<seq<uint8>>)
+    requires Materials.GetKeysFromEncryptionContext(encryptionContext) !! Materials.ReservedKeyValues
+    requires cmm.Valid() && Msg.ValidAAD(encryptionContext)
+  {
+    /*
+     * What's needed for the encryption: encryption materials, message ID, and derived data key.
+     */
+
+    var encMat :- cmm.GetEncryptionMaterials(encryptionContext, None, Some(|plaintext|));
+    if UINT16_LIMIT <= |encMat.encryptedDataKeys| {
+      return Failure("Number of EDKs exceeds the allowed maximum.");
+    }
+
+    var messageID: Msg.MessageID := Random.GenerateBytes(Msg.MESSAGE_ID_LEN as int32);
+    var derivedDataKey := DeriveKey(encMat.plaintextDataKey.get, encMat.algorithmSuiteID, messageID);
+
+    /*
+     * Assemble and serialize the header and its authentication tag.
+     */
+
+    var frameLength := 4096;
+    var headerBody := Msg.HeaderBody(
+      Msg.VERSION_1,
+      Msg.TYPE_CUSTOMER_AED,
+      encMat.algorithmSuiteID,
+      messageID,
+      encryptionContext,
+      Msg.EncryptedDataKeys(encMat.encryptedDataKeys),
+      Msg.ContentType.Framed,
+      [0, 0, 0, 0],
+      encMat.algorithmSuiteID.IVLength() as uint8,
+      frameLength);
+    var wr := new Streams.StringWriter();
+    var _ :- Serialize.SerializeHeaderBody(wr, headerBody);
+    var unauthenticatedHeader := wr.data;
+
+    var iv: seq<uint8> := seq(encMat.algorithmSuiteID.IVLength(), _ => 0);
+    var authTag :- MessageBody.Encrypt(encMat.algorithmSuiteID, iv, derivedDataKey, [], unauthenticatedHeader);
+
+    /*
+     * Encrypt the given plaintext into the message body.
+     */
+
+    var body :- MessageBody.EncryptMessageBody(plaintext, frameLength as int, messageID, derivedDataKey, encMat.algorithmSuiteID);
+
+    /*
+     * Add footer with signature, if required.
+     */
+
+    var msg := unauthenticatedHeader + authTag + body;
+
+    match encMat.algorithmSuiteID.SignatureType() {
+      case None =>
+        // don't use a footer
+      case Some(ecdsaParams) =>
+        var signResult := Signature.ECDSA.Sign(ecdsaParams, encMat.signingKey.get, msg);
+        match signResult {
+          case None =>
+            return Failure("Message signing failed");
+          case Some((r,s)) =>
+            var footer := r + s;  // TODO: this is probably not right
+            if UINT16_LIMIT <= |footer| {
+              return Failure("Signature too long");
+            }
+            msg := msg + UInt16ToSeq(|footer| as uint16) + footer;
+        }
+    }
+
+    return Success(msg);
+  }
+
+  method DeriveKey(plaintextDataKey: seq<uint8>, algorithmSuiteID: AlgorithmSuite.ID, messageID: Msg.MessageID) returns (derivedDataKey: seq<uint8>)
+    requires |plaintextDataKey| == algorithmSuiteID.KeyLength()
+    ensures |derivedDataKey| == algorithmSuiteID.KeyLength()
+  {
+    var whichSHA := AlgorithmSuite.Suite[algorithmSuiteID].hkdf;
+    if whichSHA == Digests.HmacNOSHA {
+      return plaintextDataKey;
+    }
+
+    var salt := new [0];
+    var inputKeyMaterials := SeqToArray(plaintextDataKey);
+    var infoSeq := UInt16ToSeq(algorithmSuiteID as uint16) + messageID;
+    var info := SeqToArray(infoSeq);
+    var len := algorithmSuiteID.KeyLength();
+    var derivedKey := HKDF.hkdf(whichSHA, salt, inputKeyMaterials, info, len);
+    return derivedKey[..];
+  }
+}
