Makefile
@@ -12,11 +12,15 @@ SRCS = \
 	   src/Crypto/AESEncryption.dfy \
 	   src/Crypto/Cipher.dfy \
 	   src/Crypto/Digests.dfy \
+	   src/Crypto/HKDF/CryptoMac.dfy \
+	   src/Crypto/HKDF/HKDF.dfy \
+	   src/Crypto/HKDF/HKDFSpec.dfy \
 	   src/Crypto/Random.dfy \
 	   src/Crypto/RSAEncryption.dfy \
 	   src/Crypto/Signature.dfy \
 	   src/Main.dfy \
 	   src/SDK/AlgorithmSuite.dfy \
+	   src/SDK/Client.dfy \
 	   src/SDK/CMM/DefaultCMM.dfy \
 	   src/SDK/CMM/Defs.dfy \
 	   src/SDK/Deserialize.dfy \
@@ -24,12 +28,14 @@ SRCS = \
 	   src/SDK/Keyring/Defs.dfy \
 	   src/SDK/Keyring/RSAKeyring.dfy \
 	   src/SDK/Materials.dfy \
+	   src/SDK/MessageBody.dfy \
 	   src/SDK/MessageHeader.dfy \
 	   src/SDK/Serialize.dfy \
 	   src/SDK/ToyClient.dfy \
 	   src/StandardLibrary/Base64.dfy \
 	   src/StandardLibrary/StandardLibrary.dfy \
 	   src/StandardLibrary/UInt.dfy \
+	   src/Util/Arrays.dfy \
 	   src/Util/Streams.dfy \
 	   src/Util/UTF8.dfy \
 
